Improve style

oPCF/Substitution.lean
@@ -16,19 +16,19 @@ Renaming is reflexive and transitive.
 def Ren.id' : Ren Γ Γ := fun _ ↦ id
 
 def Ren.comp (r₀₁ : Ren Γ₀ Γ₁) (r₁₂ : Ren Γ₁ Γ₂) : Ren Γ₀ Γ₂ :=
-  fun τ x => r₁₂ τ (r₀₁ τ x)
+  fun _ x => (x.ren r₀₁).ren r₁₂
 
 instance : Trans Ren Ren Ren where
   trans := Ren.comp
 
 /-
-Context extension, and hence appension, acts functorially on renamings.
+Context extension acts functorially on renamings.
 -/
 
 def Ren.keep (r : Ren Γ Δ) (τ  : Ty) : Ren (Γ ∷ τ) (Δ ∷ τ) :=
   fun υ v => match v with
-  | .z => .z
-  | .s τ x => .s τ (r τ x)
+  | .z     => .z
+  | .s _ x => (x.ren r).succ
 
 infixl:70 " ∷ᵣ "  => Ren.keep
 
@@ -39,10 +39,10 @@ theorem Ren.keep_id {Γ : Cx} (τ : Ty) : (@ Ren.id' Γ) ∷ᵣ τ = Ren.id' := 
 -- Context extension preserves the composition of renamings.
 theorem Ren.keep_comp {r₀₁ : Ren Γ₀ Γ₁} {r₁₂ : Ren Γ₁ Γ₂}
   : (r₀₁ ⬝ r₁₂) ∷ᵣ τ = (r₀₁ ∷ᵣ τ) ⬝ (r₁₂ ∷ᵣ τ) := by
-  funext τ x; cases x with | z | s => rfl
+  funext τ x; cases x with | _ => rfl
 
 def Ren.keeps (r : Ren Γ₀ Γ₁) : (Δ : Cx) → Ren (Γ₀ ++ Δ) (Γ₁ ++ Δ)
-  | .nil => r
+  | .nil      => r
   | .cons Δ τ => (r.keeps Δ).keep τ
 
 infixl:70 " ++ᵣ "  => Ren.keeps
@@ -53,17 +53,17 @@ Renaming extends to transforming terms in one context to terms in another.
 
 def Tm.ren (t : Γ ⊢ τ) (r : Ren Γ Δ) : Δ ⊢ τ :=
   match t with
-  | .var τ x => .var τ (x.ren r)
-  | .true => .true
-  | .false => .false
-  | .zero => .zero
-  | .succ e => (e.ren r).succ
-  | .pred e => (e.ren r).pred
-  | .zero? e => (e.ren r).zero?
+  | .var τ x    => (x.ren r).tm
+  | .true       => .true
+  | .false      => .false
+  | .zero       => .zero
+  | .succ e     => (e.ren r).succ
+  | .pred e     => (e.ren r).pred
+  | .zero? e    => (e.ren r).zero?
   | .cond s t f => (s.ren r).cond (t.ren r) (f.ren r)
-  | .fn e => (e.ren (r ∷ᵣ _)).fn
-  | .app f a => (f.ren r).app (a.ren r)
-  | .fix f => (f.ren r).fix
+  | .fn e       => (e.ren (r ∷ᵣ _)).fn
+  | .app f a    => (f.ren r).app (a.ren r)
+  | .fix f      => (f.ren r).fix
 
 /-
 The functoriality of context extension on renamings allows us to prove that applying the
@@ -75,10 +75,10 @@ def Tm.ren_id_eq {t : Γ ⊢ τ} : t.ren Ren.id' = t := by
   | fn e Φ =>
     calc (e.ren (Ren.id' ∷ᵣ _)).fn
       _ = (e.ren Ren.id').fn := by rw [Ren.keep_id]
-      _ = e.fn := by rw [Φ]
+      _ = e.fn               := by rw [Φ]
   | var | true | false | zero => intros; rfl
   | succ e Φ | pred e Φ | zero? e Φ | fix e Φ => exact congrArg _ Φ
-  | app f a Φf Φa => exact congrArg2 _ Φf Φa
+  | app f a Φf Φa       => exact congrArg2 _ Φf Φa
   | cond s t f Φs Φt Φf => exact congrArg3 _ Φs Φt Φf
 
 theorem Ren.ren_comp_eq {t : Γ₀ ⊢ τ}
@@ -87,15 +87,15 @@ theorem Ren.ren_comp_eq {t : Γ₀ ⊢ τ}
   | @fn _ τ υ e Φ =>
     intro _ _ r₀₁ r₁₂
     calc (e.ren ((r₀₁ ⬝ r₁₂) ∷ᵣ τ)).fn
-      _ = (e.ren ((r₀₁ ∷ᵣ τ) ⬝ (r₁₂ ∷ᵣ τ))).fn := by rw [Ren.keep_comp]
+      _ = (e.ren ((r₀₁ ∷ᵣ τ) ⬝ (r₁₂ ∷ᵣ τ))).fn   := by rw [Ren.keep_comp]
       _ = ((e.ren (r₀₁ ∷ᵣ τ)).ren (r₁₂ ∷ᵣ τ)).fn := by rw [Φ]
   | var | true | false | zero => intros; rfl
-  | succ e Φ | pred e Φ | zero? e Φ | fix e Φ => exact congrArg _ Φ
-  | app f a Φf Φa => exact congrArg2 _ Φf Φa
-  | cond s t f Φs Φt Φf => exact congrArg3 _ Φs Φt Φf
+  | succ _ Φ | pred _ Φ | zero? _ Φ | fix _ Φ => exact congrArg _ Φ
+  | app _ _ Φf Φa       => exact congrArg2 _ Φf Φa
+  | cond _ _ _ Φs Φt Φf => exact congrArg3 _ Φs Φt Φf
 
 /-
-Renaming can also be used to weaken variables in a context.
+Renaming can also be used to weaken variables in a context and rebase variables in identical contexts.
 -/
 
 def Ren.weak {τ  : Ty} : Ren Γ (Γ ∷ τ) := Var.s
@@ -105,14 +105,11 @@ theorem Ren.ren_weak_exch {r : Ren Γ₀ Γ₁} : r ⬝ Ren.weak = Ren.weak ⬝ 
   rfl
 
 def Ren.weaks : (Δ : Cx) → Ren Γ (Γ ++ Δ)
-  | .nil => id'
+  | .nil      => id'
   | .cons Δ _ => fun υ x ↦ weak υ (weaks Δ υ x)
 
-def Tm.tr_cx (t : Γ ⊢ τ) (p : Γ = Δ) : (Δ ⊢ τ) :=
-  t.ren (fun _ x ↦ x.tr_cx p)
-
-def Tm.tr_cx_rfl (t : Γ ⊢ τ) : t.tr_cx rfl = t := by
-  exact Tm.ren_id_eq
+def Ren.cast : (Γ = Δ) → Ren Γ Δ := by
+  intro p; induction p; exact Ren.id'
 
 /-
 We define substitutions on the syntax of PCF, which takes variables in one context to terms
@@ -124,26 +121,24 @@ def Subst Γ Δ := ∀ τ, Γ ∋ τ → Δ ⊢ τ
 def Var.sub (v : Γ ∋ τ) (σ : Subst Γ Δ) := σ τ v
 
 /-
-Context extension, and hence appension, acts on substitutions.
+Context extension acts on substitutions. (We leave functoriality until later.)
 -/
 
 def Subst.keep (σ : Subst Γ Δ) (τ : Ty) : Subst (Γ ∷ τ) (Δ ∷ τ) :=
   fun _ x => match x with
-  | .z => .var τ .z
-  | .s τ x => (σ τ x).ren .s
+  | .z     => .var τ .z
+  | .s _ x => (x.sub σ).ren .s
 
 infixl:70 " ∷ₛ "  => Subst.keep
 
 def Subst.keeps (σ : Subst Γ₀ Γ₁) : (Δ : Cx) → Subst (Γ₀ ++ Δ) (Γ₁ ++ Δ)
-  | .nil => σ
+  | .nil      => σ
   | .cons Δ τ => (σ.keeps Δ).keep τ
 
 infixl:70 " ++ₛ "  => Subst.keeps
 
-theorem Subst.keeps_keep_assoc (σ : Subst Γ₀ Γ₁) {Δ : Cx} (τ : Ty)
-  : (σ ++ₛ Δ) ∷ₛ τ = σ ++ₛ (Δ ∷ τ) := by
-  funext υ x
-  rfl
+theorem Subst.keeps_keep_assoc (σ : Subst Γ₀ Γ₁) {Δ : Cx} (τ : Ty) : (σ ++ₛ Δ) ∷ₛ τ = σ ++ₛ (Δ ∷ τ) := by
+  funext υ x; rfl
 
 /-
 Substitution extends to transforming terms in one context to terms in another.
@@ -151,17 +146,17 @@ Substitution extends to transforming terms in one context to terms in another.
 
 def Tm.sub (t : Γ ⊢ τ) (σ : Subst Γ Δ) : Δ ⊢ τ :=
   match t with
-  | .var _ x => x.sub σ
-  | .true => .true
-  | .false => .false
-  | .zero => .zero
-  | .succ t => (t.sub σ).succ
-  | .pred t => (t.sub σ).pred
-  | .zero? t => (t.sub σ).zero?
+  | .var _ x    => x.sub σ
+  | .true       => .true
+  | .false      => .false
+  | .zero       => .zero
+  | .succ t     => (t.sub σ).succ
+  | .pred t     => (t.sub σ).pred
+  | .zero? t    => (t.sub σ).zero?
   | .cond s t f => (s.sub σ).cond (t.sub σ) (f.sub σ)
-  | .fn e => (e.sub (σ ∷ₛ _)).fn
-  | .app f a => (f.sub σ).app (a.sub σ)
-  | .fix f => (f.sub σ).fix
+  | .fn e       => (e.sub (σ ∷ₛ _)).fn
+  | .app f a    => (f.sub σ).app (a.sub σ)
+  | .fix f      => (f.sub σ).fix
 
 /-
 Substitution is reflexive and transitive.
@@ -170,7 +165,7 @@ Substitution is reflexive and transitive.
 def Subst.id' : Subst Γ Γ := fun τ x => .var τ x
 
 def Subst.comp (σ₀₁ : Subst Γ₀ Γ₁) (σ₁₂ : Subst Γ₁ Γ₂) : Subst Γ₀ Γ₂ :=
-  fun τ x => (σ₀₁ τ x).sub σ₁₂
+  fun _ x => (x.sub σ₀₁).sub σ₁₂
 
 instance : Trans Subst Subst Subst where
   trans := Subst.comp
@@ -179,14 +174,8 @@ def Subst.weak {υ : Ty} : Subst Γ (Γ ∷ υ):=
   fun _ x => x.succ.tm
 
 /-
-Our next goal is to show that context extension acts functorially on substitutions (that is,
-preserves identity and composition). This is surprisingly involved, as you're about to see.
+Substitution and weakening commute. This takes a decent amount of preparation to prove.
 -/
-
--- Context extension preserves the identity substitution.
-def Subst.keep_id : (@ Subst.id' Γ) ∷ₛ τ = Subst.id' := by
-  funext τ x
-  cases x with | z | s => rfl
 
 -- The following lemmas allow manipulating variables and renamings in the presence of type casts.
 def cx_eq_cons {Γ Δ : Cx} (p : Γ = Δ) (υ : Ty) : Γ ∷ υ = Δ ∷ υ := by
@@ -198,107 +187,90 @@ def cx_comp_eq_cx {Γ Δ : Cx} (h : Γ ∷ τ = Δ ∷ υ) : Γ = Δ := by
 def cx_comp_eq_ty {Γ Δ : Cx} (h : Γ ∷ τ = Δ ∷ υ) : τ = υ := by
   cases h with | refl => rfl
 
-def Var.tr_cx_z
-  (h : Γ ∷ υ = Δ ∷ υ) : (Var.z).tr_cx h = Var.z := by
+def Tm.ren_cast_rfl (t : Γ ⊢ τ) : t.ren (Ren.cast rfl) = t := Tm.ren_id_eq
+
+def Var.ren_cast_z (h : Γ ∷ υ = Δ ∷ υ) : (Var.z).ren (Ren.cast h) = Var.z := by
   cases h with | refl => rfl
 
-def Var.tr_cx_s
-  (h : Γ = Δ) : (Var.s τ x).tr_cx (cx_eq_cons h υ) = Var.s τ (x.tr_cx h) := by
+def Var.ren_cast_s (h : Γ = Δ)
+  : (Var.s τ x).ren (Ren.cast (cx_eq_cons h υ)) = Var.s τ (x.ren (Ren.cast h)) := by
   cases h with | refl => rfl
 
-def keep_tr_cx
-  : ((fun _ x ↦ x.tr_cx h) ∷ᵣ υ : Ren (Γ ∷ υ) (Δ ∷ υ)) = fun _ x ↦ x.tr_cx (cx_eq_cons h υ) := by
-  funext τ x
-  induction h with | refl => cases x with | z | s => rfl
+def Ren.cast_keep_eq
+  : (Ren.cast h ∷ᵣ υ : Ren (Γ ∷ υ) (Δ ∷ υ)) = Ren.cast (cx_eq_cons h υ) := by
+  funext τ x; induction h with | refl => cases x with | _ => rfl
 
 -- Shorthand for weakening with an arbitrary context appension.
 def weak' {Γ} {τ} {Δ} : Ren (Γ ++ Δ) (Γ ∷ τ ++ Δ) := Ren.weak ++ᵣ Δ
 
 -- The application of substitution and generalized weakening commutes on variables.
 def sub_weak'_exchange_var {Δ} : ∀ {Γ} {Γ₀ Γ₁ : Cx} {σ : Subst Γ₀ Γ₁} {τ'} {h : Γ = Γ₀ ++ Δ} {ν} {x : Γ ∋ ν},
-    (((x.tr_cx h).ren (Ren.id' ++ᵣ Δ)).sub (σ ++ₛ Δ)).ren weak'
-  = (((x.tr_cx h).ren (Ren.id' ++ᵣ Δ)).ren weak').sub ((σ ∷ₛ τ') ++ₛ Δ)
-    := by
-    induction Δ with
-    | nil => intros; rfl
-    | cons Δ τ Φ =>
-      intro Γ Γ₀ Γ₁ σ τ' h ν x
-      cases x with
-      | @z ν Γ => induction cx_comp_eq_ty h with | refl => rw [Var.tr_cx_z]; rfl
-      | @s Γ υ ν x =>
-        induction cx_comp_eq_ty h with
-        | refl =>
-          rw [Var.tr_cx_s (cx_comp_eq_cx h)]
-          let y := ((x.tr_cx (cx_comp_eq_cx h))).ren (Ren.id' ++ᵣ Δ)
-          calc  (y.succ.sub (σ ++ₛ (Δ ∷ υ))).ren weak'
-            _ = ((y.sub (σ ++ₛ Δ)).ren Ren.weak).ren (weak' ∷ᵣ υ)     := rfl
-            _ = (y.sub (σ ++ₛ Δ)).ren (Ren.weak ⬝ (weak' ∷ᵣ υ))       := by rw [Ren.ren_comp_eq]
-            _ = (y.sub (σ ++ₛ Δ)).ren (weak' ⬝ Ren.weak)              := by rw [Ren.ren_weak_exch]
-            _ = ((y.sub (σ ++ₛ Δ)).ren weak').ren Ren.weak            := by rw [Ren.ren_comp_eq]
-            _ = ((y.ren weak').sub ((σ ∷ₛ τ') ++ₛ Δ)).ren Ren.weak    := by rw [Φ]
-            _ = (y.succ.ren (weak' ∷ᵣ υ)).sub (σ ∷ₛ τ' ++ₛ (Δ ∷ υ)) := rfl
+    (((x.ren (Ren.cast h)).ren (Ren.id' ++ᵣ Δ)).sub (σ ++ₛ Δ)).ren weak'
+  = (((x.ren (Ren.cast h)).ren (Ren.id' ++ᵣ Δ)).ren weak').sub ((σ ∷ₛ τ') ++ₛ Δ)
+  := by
+  induction Δ with
+  | nil => intros; rfl
+  | cons Δ τ Φ =>
+    intro Γ Γ₀ Γ₁ σ τ' h ν x
+    cases x with
+    | z => induction cx_comp_eq_ty h with | refl => rw [Var.ren_cast_z]; rfl
+    | @s Γ υ _ x =>
+      induction cx_comp_eq_ty h with
+      | refl =>
+        rw [Var.ren_cast_s (cx_comp_eq_cx h)]
+        let y := ((x.ren (Ren.cast (cx_comp_eq_cx h)))).ren (Ren.id' ++ᵣ Δ)
+        calc  (y.succ.sub (σ ++ₛ (Δ ∷ υ))).ren weak'
+          _ = ((y.sub (σ ++ₛ Δ)).ren Ren.weak).ren (weak' ∷ᵣ υ)     := rfl
+          _ = (y.sub (σ ++ₛ Δ)).ren (Ren.weak ⬝ (weak' ∷ᵣ υ))       := by rw [Ren.ren_comp_eq]
+          _ = (y.sub (σ ++ₛ Δ)).ren (weak' ⬝ Ren.weak)              := by rw [Ren.ren_weak_exch]
+          _ = ((y.sub (σ ++ₛ Δ)).ren weak').ren Ren.weak            := by rw [Ren.ren_comp_eq]
+          _ = ((y.ren weak').sub ((σ ∷ₛ τ') ++ₛ Δ)).ren Ren.weak    := by rw [Φ]
+          _ = (y.succ.ren (weak' ∷ᵣ υ)).sub (σ ∷ₛ τ' ++ₛ (Δ ∷ υ))   := rfl
 
 -- The application of substitution and generalized weakening commutes on terms.
 def sub_weak'_exchange_tm {t : Γ ⊢ τ} : ∀ Δ {Γ₀ Γ₁ : Cx} {h : Γ = Γ₀ ++ Δ} {σ : Subst Γ₀ Γ₁} {τ'},
-    (((t.tr_cx h).ren (Ren.id' ++ᵣ Δ)).sub (σ ++ₛ Δ)).ren weak'
-  = (((t.tr_cx h).ren (Ren.id' ++ᵣ Δ)).ren weak').sub ((σ ∷ₛ τ') ++ₛ Δ)
+    (((t.ren (Ren.cast h)).ren (Ren.id' ++ᵣ Δ)).sub (σ ++ₛ Δ)).ren weak'
+  = (((t.ren (Ren.cast h)).ren (Ren.id' ++ᵣ Δ)).ren weak').sub ((σ ∷ₛ τ') ++ₛ Δ)
   := by
   induction t with
-  -- If `t` is a variable, this is exactly our variable exchange assumption.
-  | var υ x =>
-    intro Δ Γ₀ Γ₁ h σ τ'
-    show ((((x.tr_cx h).ren (Ren.id' ++ᵣ Δ))).sub (σ ++ₛ Δ)).ren weak'
-       = ((((x.tr_cx h).ren (Ren.id' ++ᵣ Δ))).ren weak').sub ((σ ∷ₛ τ') ++ₛ (Δ))
-    rw [sub_weak'_exchange_var]
-  -- If `t` is a function `e.fn`, we must prove our variable exchange assumption for a weakened context,
-  -- allowing the induction hypothesis to be applied for the function body `e`.
   | @fn Γ' υ τ e Φ =>
     intro Δ Γ₀ Γ₁ h σ τ'
-    calc (((e.fn.tr_cx h).ren (Ren.id' ++ᵣ Δ)).sub (σ ++ₛ Δ)).ren weak'
-      _ = ((((e.ren ((fun _ x ↦ x.tr_cx h) ∷ᵣ υ)).ren (Ren.id' ++ᵣ (Δ ∷ υ))).sub
-        (σ ++ₛ (Δ ∷ υ))).ren (weak'.keep _)).fn := rfl
-      _ = ((((e.ren (fun _ x ↦ x.tr_cx (cx_eq_cons h υ))).ren (Ren.id' ++ᵣ (Δ ∷ υ))).sub
-        ((σ ++ₛ (Δ ∷ υ)))).ren (weak'.keep _)).fn := by rw [keep_tr_cx]
-      _ = ((((e.tr_cx (cx_eq_cons h υ)).ren (Ren.id' ++ᵣ (Δ ∷ υ))).sub (σ ++ₛ (Δ ∷ υ))).ren
-        (weak'.keep _)).fn := rfl
-      _ = ((((e.tr_cx (cx_eq_cons h υ)).ren (Ren.id' ++ᵣ (Δ ∷ υ))).ren (weak'.keep _)).sub
-        ((σ.keep τ') ++ₛ (Δ ∷ υ))).fn := by congr; apply Φ (Δ ∷ υ)
-      _ = ((((e.ren (fun _ x ↦ x.tr_cx (cx_eq_cons h υ))).ren ((Ren.id' ++ᵣ Δ).keep _)).ren
-        (weak'.keep _)).sub (((σ.keep τ') ++ₛ Δ).keep υ)).fn := rfl
-      _ = ((((e.ren (Ren.keep (fun _ x ↦ x.tr_cx h) _)).ren ((Ren.id' ++ᵣ Δ).keep _)).ren
-        (weak'.keep _)).sub (((σ.keep τ') ++ₛ Δ).keep υ)).fn := by rw [keep_tr_cx]
-      _ =  (((e.fn.tr_cx h).ren (Ren.id' ++ᵣ Δ)).ren weak').sub (σ ∷ₛ τ' ++ₛ Δ) := rfl
+    let y₀ := ((e.ren (Ren.cast h ∷ᵣ υ)).ren (Ren.id' ++ᵣ (Δ ∷ υ)))
+    let y₁ := ((e.ren (Ren.cast (cx_eq_cons h υ))).ren (Ren.id' ++ᵣ (Δ ∷ υ)))
+    show ((y₀.sub _).ren _).fn = ((y₀.ren _).sub _).fn
+    dsimp [y₀]; rw [Ren.cast_keep_eq]
+    show ((y₁.sub _).ren _).fn = ((y₁.ren _).sub _).fn
+    congr
+    exact Φ (Δ ∷ υ)
+  | var υ x => intros; exact sub_weak'_exchange_var
   | true | false | zero => intros; rfl
-  | succ e Φ | pred e Φ | zero? e Φ | fix e Φ =>
-    intro _ _ _ _ _ _
-    exact congrArg _ (Φ _)
-  | app f a Φf Φa =>
-    intro _ _ _ _ _ _
-    exact congrArg2 _ (Φf _) (Φa _)
-  | cond s t f Φs Φt Φf =>
-    intro _ _ _ _ _ _
-    exact congrArg3 _ (Φs _) (Φt _) (Φf _)
+  | succ _ Φ | pred _ Φ | zero? _ Φ | fix _ Φ => intros; exact congrArg _ (Φ _)
+  | app _ _ Φf Φa       => intros; exact congrArg2 _ (Φf _) (Φa _)
+  | cond _ _ _ Φs Φt Φf => intros; exact congrArg3 _ (Φs _) (Φt _) (Φf _)
 
 -- The application of substitution and weakening commutes on terms.
 def sub_weak_exchange {t : Γ₀ ⊢ τ} {σ : Subst Γ₀ Γ₁}  : (t.sub σ).ren .s = (t.ren .s).sub (σ ∷ₛ υ) := by
-    have p
-      : ((((t.tr_cx rfl).ren ((Ren.weaks Cx.nil) ++ᵣ Cx.nil)).sub (σ ++ₛ (Cx.nil ++ Cx.nil))).ren .s)
-      = (((t.tr_cx rfl).ren ((Ren.weaks Cx.nil) ++ᵣ Cx.nil)).ren .s).sub ((σ ∷ₛ υ) ++ₛ (Cx.nil ++ Cx.nil))
-      := @sub_weak'_exchange_tm Γ₀ τ t Cx.nil Γ₀ Γ₁ rfl σ υ
-    rw [Tm.tr_cx_rfl] at p
-    change ((t.ren Ren.id').sub σ).ren .s = ((t.ren Ren.id').ren .s).sub (σ ∷ₛ υ) at p
+    have p := @sub_weak'_exchange_tm Γ₀ τ t Cx.nil Γ₀ Γ₁ rfl σ υ
+    rw [Tm.ren_cast_rfl] at p
+    change ((t.ren Ren.id').sub _).ren _ = ((t.ren Ren.id').ren _).sub _ at p
     rw [Tm.ren_id_eq] at p
     exact p
+
+/-
+Context extension acts functorially on substitutions.
+-/
+
+-- Context extension preserves the identity substitution.
+def Subst.keep_id : (@ Subst.id' Γ) ∷ₛ τ = Subst.id' := by
+  funext _ x; cases x with | _ => rfl
 
 -- Context extension preserves the composition of substitutions.
 def Subst.keep_comp {σ₀₁ : Subst Γ₀ Γ₁} {σ₁₂ : Subst Γ₁ Γ₂}
   : (σ₀₁ ⬝ σ₁₂) ∷ₛ τ = (σ₀₁ ∷ₛ τ) ⬝ (σ₁₂ ∷ₛ τ) := by
   funext υ x
   cases x with
-  | z => calc Var.z.tm = Var.z.tm := rfl
-  | s υ x =>
-    show ((σ₀₁ υ x).sub σ₁₂).ren .s = ((σ₀₁ υ x).ren .s).sub (σ₁₂ ∷ₛ τ)
-    exact sub_weak_exchange
+  | z => rfl
+  | s => exact sub_weak_exchange
 
 /-
 The functoriality of context extension on substitutions allows us to prove that applying the
@@ -308,84 +280,83 @@ identity substitution and composite substitutions to a term does exactly what we
 def Tm.sub_id_eq {t : Γ ⊢ τ} : t.sub (Subst.id') = t := by
   induction t with
   | fn e Φ =>
-    calc e.fn.sub Subst.id'
+    calc  e.fn.sub Subst.id'
       _ = (e.sub (Subst.id' ∷ₛ _)).fn := rfl
       _ = (e.sub Subst.id').fn        := by rw [Subst.keep_id]
       _ = e.fn                        := by rw [Φ]
-  | var | true | false | zero => rfl
+  | var | true | false | zero                 => rfl
   | succ e Φ | pred e Φ | zero? e Φ | fix e Φ => exact congrArg _ Φ
-  | app f a Φf Φa => exact congrArg2 _ Φf Φa
-  | cond s t f Φs Φt Φf => apply congrArg3 _ Φs Φt Φf
+  | app f a Φf Φa                             => exact congrArg2 _ Φf Φa
+  | cond s t f Φs Φt Φf                       => apply congrArg3 _ Φs Φt Φf
 
 def Tm.sub_comp_eq {t : Γ₀ ⊢ τ}
   : ∀ {Γ₁ Γ₂} {σ₀₁ : Subst Γ₀ Γ₁} {σ₁₂ : Subst Γ₁ Γ₂}, t.sub (σ₀₁ ⬝ σ₁₂) = (t.sub σ₀₁).sub σ₁₂ := by
   induction t with
-  | @fn _ τ υ e Φ =>
+  | @fn _ τ _ e Φ =>
     intro _ _ σ₀₁ σ₁₂
-    calc e.fn.sub (σ₀₁ ⬝ σ₁₂)
+    calc   e.fn.sub (σ₀₁ ⬝ σ₁₂)
       _ = (e.sub ((σ₀₁ ⬝ σ₁₂) ∷ₛ τ)).fn          := rfl
       _ = (e.sub ((σ₀₁ ∷ₛ τ) ⬝ (σ₁₂ ∷ₛ τ))).fn   := by rw [Subst.keep_comp]
       _ = ((e.sub (σ₀₁ ∷ₛ τ)).sub (σ₁₂ ∷ₛ τ)).fn := by rw [Φ]
       _ = (e.fn.sub σ₀₁).sub σ₁₂                 := rfl
-  | var | true | false | zero => intros; rfl
-  | succ e Φ | pred e Φ | zero? e Φ | fix e Φ => exact congrArg _ Φ
-  | app f a Φf Φa => exact congrArg2 _ Φf Φa
-  | cond s t f Φs Φt Φf => exact congrArg3 _ Φs Φt Φf
+  | var | true | false | zero                 => intros; rfl
+  | succ e Φ | pred e Φ | zero? e Φ | fix e Φ => exact congrArg  _ Φ
+  | app f a Φf Φa                             => exact congrArg2 _ Φf Φa
+  | cond s t f Φs Φt Φf                       => exact congrArg3 _ Φs Φt Φf
 
 /-
-Instantiation is dual to weakening, and
+Lastly, we directly characterize `keep` composed with `inst` as 'pushing' a term onto a substitution.
 -/
 
-def Subst.inst : (t : Γ ⊢ τ) → Subst (Γ ∷ τ) Γ :=
-  fun a τ x => match x with
-  | .z => a
-  | .s τ x => .var τ x
-
-def Subst.amend (σ : Subst Γ₁ Γ₂) (r : Ren Γ₀ Γ₁) : Subst Γ₀ Γ₂ :=
-  fun τ x => σ τ (r τ x)
-
 def Subst.push (σ : Subst Γ Δ) {υ : Ty} (a : Δ ⊢ υ) : Subst (Γ ∷ υ) Δ :=
-  fun τ x => match x with
-  | .z => a
-  | .s τ x => σ τ x
+  fun _ x => match x with
+  | .z     => a
+  | .s _ x => x.sub σ
 
-def sub_amend_keep_eq {r : Ren Γ₀ Γ₁} {σ : Subst Γ₁ Γ₂}
-  : (σ.amend r) ∷ₛ τ = ((σ ∷ₛ τ).amend (r ∷ᵣ τ)) := by
-  funext τ x
-  cases x with
-  | z | s => rfl
+def Ren.then (r : Ren Γ₀ Γ₁) (σ : Subst Γ₁ Γ₂) : Subst Γ₀ Γ₂ :=
+  fun _ x => (x.ren r).sub σ
 
-def sub_amend_eq {t : Γ₀ ⊢ τ}
-  : ∀ {Γ₁ Γ₂} {r : Ren Γ₀ Γ₁} {σ : Subst Γ₁ Γ₂}, (t.ren r).sub σ = t.sub (σ.amend r) := by
+instance : Trans Ren Subst Subst where
+  trans := Ren.then
+
+def Subst.inst : (t : Γ ⊢ τ) → Subst (Γ ∷ τ) Γ :=
+  fun a _ x => match x with
+  | .z     => a
+  | .s _ x => x.tm
+
+def Subst.keep_then_eq {r : Ren Γ₀ Γ₁} {σ : Subst Γ₁ Γ₂} : (r ⬝ σ) ∷ₛ τ = ((r ∷ᵣ τ) ⬝ (σ ∷ₛ τ)) := by
+  funext τ x; cases x with | _ => rfl
+
+def Tm.sub_then_eq {t : Γ₀ ⊢ τ}
+  : ∀ {Γ₁ Γ₂} {r : Ren Γ₀ Γ₁} {σ : Subst Γ₁ Γ₂}, t.sub (r ⬝ σ) = (t.ren r).sub σ := by
   induction t with
   | fn e Φ =>
     intro _ _ r σ
-    calc (e.fn.ren r).sub σ
-      _ = (((e.ren (r ∷ᵣ _)).sub (σ ∷ₛ _)).fn) := rfl
-      _ = ((e.sub ((σ ∷ₛ _).amend (r ∷ᵣ _))).fn) := by rw [Φ]
-      _ = ((e.sub ((σ.amend r) ∷ₛ _)).fn) := by rw [sub_amend_keep_eq]
-      _ = e.fn.sub (σ.amend r) := rfl
-  | var | true | false | zero => intros; rfl
-  | succ e Φ | pred e Φ | zero? e Φ | fix e Φ => exact congrArg _ Φ
-  | app f a Φf Φa => exact congrArg2 _ Φf Φa
-  | cond s t f Φs Φt Φf => exact congrArg3 _ Φs Φt Φf
+    calc  e.fn.sub (r ⬝ σ)
+      _ = ((e.sub ((r ⬝ σ) ∷ₛ _)).fn)          := rfl
+      _ = ((e.sub ((r ∷ᵣ _) ⬝ (σ ∷ₛ _))).fn)   := by rw [Subst.keep_then_eq]
+      _ = (((e.ren (r ∷ᵣ _)).sub (σ ∷ₛ _)).fn) := by rw [Φ]
+      _ = (e.fn.ren r).sub σ                   := rfl
+  | var | true | false | zero                 => intros; rfl
+  | succ e Φ | pred e Φ | zero? e Φ | fix e Φ => exact congrArg  _ Φ
+  | app f a Φf Φa                             => exact congrArg2 _ Φf Φa
+  | cond s t f Φs Φt Φf                       => exact congrArg3 _ Φs Φt Φf
 
-def inst_amend_weak_eq_id : (Subst.inst a).amend .s = Subst.id' := by
-  funext τ x
-  cases x with | z | s => rfl
+def Subst.weak_inst_eq : Ren.weak ⬝ (Subst.inst a) = Subst.id' := by
+  funext _ x; cases x with | _ => rfl
 
-def ren_weak_sub_inst_eq {t : Γ ⊢ τ} : (t.ren .s).sub (Subst.inst a) = t := by
-  calc (t.ren .s).sub (Subst.inst a)
-    _ = t.sub ((Subst.inst a).amend .s) := by rw [sub_amend_eq]
-    _ = t.sub (Subst.id')               := by rw [inst_amend_weak_eq_id]
-    _ = t                               := by rw [Tm.sub_id_eq]
+def Tm.weak_inst_eq {t : Γ ⊢ τ} : (t.ren .s).sub (Subst.inst a) = t := by
+  calc (t.ren Ren.weak).sub (Subst.inst a)
+    _ = t.sub (Ren.weak ⬝ (Subst.inst a)) := by rw [Tm.sub_then_eq]
+    _ = t.sub (Subst.id')                 := by rw [Subst.weak_inst_eq]
+    _ = t                                 := by rw [Tm.sub_id_eq]
 
-def sub_push_eq_keep_inst {σ : Subst  Γ Δ} {υ : Ty} {a : Δ ⊢ υ} : σ.push a = (σ ∷ₛ υ) ⬝ Subst.inst a := by
-  funext τ x
+def Subst.push_eq {σ : Subst  Γ Δ} {υ : Ty} {a : Δ ⊢ υ} : σ.push a = (σ ∷ₛ υ) ⬝ Subst.inst a := by
+  funext _ x
   cases x with
-  | z => rfl
-  | s τ x =>
-    calc σ.push a τ x.s
-      _ = σ τ x := rfl
-      _ = ((σ τ x).ren .s).sub (Subst.inst a) := by rw [ren_weak_sub_inst_eq]
-      _ = ((σ ∷ₛ υ) ⬝ Subst.inst a) τ x.s     := rfl
+  | z     => rfl
+  | s _ x =>
+    calc  x.succ.sub (σ.push a)
+      _ = x.sub σ                               := rfl
+      _ = ((x.sub σ).ren .s).sub (Subst.inst a) := by rw [Tm.weak_inst_eq]
+      _ = x.succ.sub ((σ ∷ₛ υ) ⬝ Subst.inst a)  := rfl
