oPCF/Operation.lean
@@ -1,5 +1,9 @@
 import «oPCF».Substitution
 
+/-
+The 'big-step' operational semantics of PCF characterizes the results of terms.
+-/
+
 inductive Eval : (.nil ⊢ τ) → (.nil ⊢ τ) → Type
   | true : Eval .true .true
   | false : Eval .false .false
@@ -16,18 +20,17 @@ inductive Eval : (.nil ⊢ τ) → (.nil ⊢ τ) → Type
 
 infixl:75 " ⇓ " => Eval
 
--- Proposition 23 (Determinism)
-theorem determinism : t ⇓ v₀ → t ⇓ v₁ → v₀ = v₁ := by
+/-
+Evaluation is deterministic: evaluation results are unique.
+-/
+
+theorem Eval.determinism : t ⇓ v₀ → t ⇓ v₁ → v₀ = v₁ := by
   intro h₀ h₁
   induction h₀ with
-  | true | false | zero | fn =>
-    cases h₁
-    rfl
+  | true | false | zero | fn => cases h₁; rfl
   | succ _ Φ =>
-    cases h₁
-    case _ _ x =>
-    congr
-    exact Φ x
+    cases h₁ with
+    | succ x => congr; exact Φ x
   | pred _ _ Φ =>
     cases h₁ with
     | pred _ x => injection Φ x
@@ -48,12 +51,29 @@ theorem determinism : t ⇓ v₀ → t ⇓ v₁ → v₀ = v₁ := by
     | cond_true x₀ => injection Φ₀ x₀
     | cond_false _ x₁ => exact Φ₁ x₁
   | app _ _ Φ₀ Φ₁ =>
-    cases h₁
-    case _ x₀ x₁ =>
-    injection Φ₀ x₀ with _ _ _ p
-    rw [←p] at x₁
-    exact Φ₁ x₁
+    cases h₁ with
+    | app  x₀ x₁ =>
+      injection Φ₀ x₀ with _ _ _ p
+      rw [← p] at x₁
+      exact Φ₁ x₁
   | fix _ Φ =>
-    cases h₁
-    case fix x₀ =>
-    exact Φ x₀
+    cases h₁ with
+    | fix x₀ => exact Φ x₀
+
+/-
+Evaluation results are values.
+-/
+
+def Eval.value : (t ⇓ v) → v.is_value
+  | .true | .false | .zero | .fn | .zero?_zero .. | .zero?_succ .. => by constructor
+  | succ e   => e.value.succ
+  | pred v _ => v
+  | .cond_true _ e | .cond_false _ e | .app _ e | .fix e => e.value
+
+/-
+Any value evaluates to itself.
+-/
+
+def Tm.is_value.self_evaluates : v.is_value → (v ⇓ v)
+  | .true | .false | .zero | .fn => by constructor
+  | .succ n => .succ n.self_evaluates
